fixing small-step

deps/poulet4/lib/P4cub/Semantics/Dynamic/SmallStep/Util.v
@@ -1,501 +1,396 @@
-Set Warnings "-custom-entry-overridden".
 Require Import Poulet4.P4cub.Syntax.Syntax
         Poulet4.P4cub.Semantics.Dynamic.SmallStep.Value
         Poulet4.P4cub.Semantics.Climate Poulet4.Utils.P4Arith
         Coq.PArith.BinPos Coq.ZArith.BinInt Coq.NArith.BinNat
         Coq.Arith.Compare_dec Coq.micromega.Lia
-        Poulet4.P4cub.Semantics.Static.Static.
-Import String.
+        Poulet4.P4cub.Semantics.Static.Static
+        Poulet4.Utils.ForallMap.
 
 Section StepDefs.
-  Import TypeEquivalence ProperType
-         F.FieldTactics P4ArithTactics
-         AllCubNotations Clmt.Notations.
-  
-  Context {tags_t : Type}.
-  
-  (** Expression environment. *)
-  Definition eenv : Type := Clmt.t (string) (Expr.e tags_t).
+  Import P4ArithTactics AllCubNotations.
   
   (** Bit-slicing. *)
-  Definition eval_slice (hi lo : positive) (v : Expr.e tags_t) : option (Expr.e tags_t) :=
+  Definition eval_slice (hi lo : positive) (v : Expr.e) : option Expr.e :=
     match v with
-    | <{ _ W z @ i }>
-    | <{ _ S z @ i }>
-      => let w' := (hi - lo + 1)%positive in
-        Some $ Expr.EBit (Npos w')
-             (BitArith.mod_bound (Npos w') $
-              BitArith.bitstring_slice z hi lo) i
+    | (_ `W z)%expr
+    | (_ `S z)%expr
+      => let w' := (Npos hi - Npos lo + 1)%N in
+        Some $ Expr.Bit w'
+             (BitArith.mod_bound
+                w' $ BitArith.bitstring_slice z hi lo)
     | _ => None
     end.
-  (**[]*)
   
   Definition eval_cast
-             (target : Expr.t) (v : Expr.e tags_t) : option (Expr.e tags_t) :=
+             (target : Expr.t) (v : Expr.e) : option Expr.e :=
     match target, v with
-    | (Expr.TBit (Npos 1)), <{ TRUE @ i }>         => Some (Expr.EBit 1%N 1%Z i)
-    | (Expr.TBit (Npos 1)), <{ FALSE @ i }>        => Some (Expr.EBit 1%N 0%Z i)
-    | {{ Bool }}, Expr.EBit 1%N 1%Z i => Some <{ TRUE @ i }>
-    | {{ Bool }}, Expr.EBit 1%N 0%Z i => Some <{ FALSE @ i }>
-    | {{ bit<w> }}, Expr.EInt _ z i
-      => let n := BitArith.mod_bound w z in
-        Some <{ w W n @ i }>
-    | {{ int<w> }}, <{ _ W n @ i }>
-      => let z := IntArith.mod_bound w n in
-        Some <{ w S z @ i }>
-    | {{ bit<w> }}, <{ _ W n @ i }>
-      => let n := BitArith.mod_bound w n in
-        Some <{ w W n @ i }>
-    | {{ int<w> }}, <{ _ S z @ i}>
-      => let z := IntArith.mod_bound w z in
-        Some <{ w S z @ i }>
-    | {{ struct { fs } }}, <{ tup vs @ i }>
-      => Some $ Expr.EStruct (combine (F.keys fs) vs) i
-    | {{ hdr { fs } }}, <{ tup vs @ i }>
-      => Some
-          $ Expr.EHeader
-          (combine (F.keys fs) vs) <{ TRUE @ i }> i
+    | Expr.TBit (Npos 1), Expr.Bool true => Some $ Expr.Bit 1%N 1%Z
+    | Expr.TBit (Npos 1), Expr.Bool false => Some $ Expr.Bit 1%N 0%Z
+    | Expr.TBool, Expr.Bit 1%N 1%Z=> Some $ Expr.Bool true
+    | Expr.TBool, Expr.Bit 1%N 0%Z=> Some $ Expr.Bool true
+    | Expr.TBit w, (_ `S z)%expr
+      => Some $ Expr.Bit w $ BitArith.mod_bound w z
+    | Expr.TInt w, (_ `W n)%expr
+      => Some $ Expr.Int w $ IntArith.mod_bound w n
+    | Expr.TBit w, (_ `W n)%expr
+      => Some $ Expr.Bit w $ BitArith.mod_bound w n
+    | Expr.TInt w, (_ `S z)%expr
+      => Some $ Expr.Int w $ IntArith.mod_bound w z
+    | Expr.TStruct _ true, Expr.Struct vs _
+      => Some $ Expr.Struct vs (Some true)
     | _, _ => None
     end.
-  (**[]*)
   
   (** Default (value) Expression. *)
-  Fail Fixpoint edefault (i : tags_t) (τ : Expr.t) : Expr.e tags_t :=
-    let fix lstruct (ts : list (Expr.t)) : list (Expr.e tags_t) :=
-        match ts with
-        | []     => []
-        | τ :: ts => edefault i τ :: lstruct ts
-        end in
-    let fix fstruct (fs : F.fs string (Expr.t))
-        : F.fs string (Expr.t * Expr.e tags_t) :=
-        match fs with
-        | [] => []
-        | (x, τ) :: fs => (x, edefault i τ) :: fstruct fs
-        end in
+  Fixpoint e_of_t (τ : Expr.t) : option Expr.e :=
     match τ with
-    | {{ Bool }} => <{ BOOL false @ i }>
-    | {{ bit<w> }} => Expr.EBit w 0%Z i
-    | {{ int<w> }} => Expr.EInt w 0%Z i
-    | {{ error }} => <{ Error None @ i }>
-    | {{ tuple ts }} => Expr.ETuple (lstruct ts) i
-    | {{ struct { fs } }} => Expr.EStruct (fstruct fs) i
-    | {{ hdr { fs } }} => Expr.EHeader (fstruct fs) <{ BOOL false @ i }> i
-    | {{ stack tfs[n] }}
-      => let tefs := fstruct tfs in
-        let hs :=
-            repeat
-            <{ hdr { tefs } valid:= BOOL false @ i @ i }>
-            (Pos.to_nat n) in
-        Expr.EHeaderStack tfs hs n 0%Z i
+    | Expr.TBool => Some $ Expr.Bool false
+    | Expr.TBit w => Some $ Expr.Bit w 0%Z
+    | Expr.TInt w => Some $ Expr.Int w 0%Z
+    | Expr.TError => Some $ Expr.Error None
+    | Expr.TStruct τs b =>
+        let^ es := sequence $ List.map e_of_t τs in
+        Expr.Struct es (if b then Some false else None)
+    | Expr.TVar _ => None
     end.
-  (**[]*)
   
   (** Unary Operations. *)
-  Definition eval_uop (op : Expr.uop) (e : Expr.e tags_t) : option (Expr.e tags_t) :=
+  Definition eval_uop (op : Expr.uop) (e : Expr.e) : option Expr.e :=
     match op, e with
-    | _{ ! }_, <{ BOOL b @ i }>
-      => let b' := negb b in Some <{ BOOL b' @ i }>
-    | _{ ~ }_, <{ w W n @ i }>
-      => let n' := BitArith.bit_not w n in Some <{ w W n' @ i }>
-    | _{ ~ }_, <{ w S n @ i }>
-      => let n' := IntArith.bit_not w n in Some <{ w S n' @ i }>
-    | _{ - }_, <{ w W z @ i }>
-      => let z' := BitArith.neg w z in Some <{ w W z' @ i }>
-    | _{ - }_, <{ w S z @ i }>
-      => let z' := IntArith.neg w z in Some <{ w S z' @ i }>
-    | _{ isValid }_, <{ hdr { _ } valid:=b @ i }> => Some b
-    | _{ setValid }_, <{ hdr { fs } valid:=_ @ i }>
-      => Some <{ hdr { fs } valid:=TRUE @ i @ i}>
-    | _{ setInValid }_, <{ hdr { fs } valid:=b @ i }>
-      => Some <{ hdr { fs } valid:=FALSE @ i @ i }>
-    | _{ Size }_, <{ Stack _:_ nextIndex:=_ @ i }>
-      => let w := 32%N in
-        (* XXX need actual size instead of 0 here *)
-        let s := Zpos xH in Some <{ w W s @ i }>
-    | _{ Next }_, <{ Stack hs:_ nextIndex:=ni @ _ }>
-      => nth_error hs $ Z.to_nat ni
+    | `!%uop, (Expr.Bool b) => Some (Expr.Bool $ negb b)
+    | `~%uop, (w `W n)%expr => Some $ Expr.Bit w $ BitArith.bit_not w n
+    | `~%uop, (w `S n)%expr => Some $ Expr.Int w $ IntArith.bit_not w n
+    | `-%uop, (w `W z)%expr => Some $ Expr.Bit w $ BitArith.neg w z
+    | `-%uop, (w `S z)%expr => Some $ Expr.Int w $ IntArith.neg w z
+    | Expr.IsValid, Expr.Struct _ (Some b) => Some $ Expr.Bool b
+    | Expr.SetValidity b, Expr.Struct fs _
+      => Some $ Expr.Struct fs $ Some b
     | _, _ => None
     end.
-  (**[]*)
+
+  Local Open Scope expr_scope.
   
   (** Binary operations. *)
   Definition eval_bop
-             (op : Expr.bop) (v1 v2 : Expr.e tags_t) (i : tags_t) : option (Expr.e tags_t) :=
+             (op : Expr.bop) (v1 v2 : Expr.e) : option Expr.e :=
     match op, v1, v2 with
-    | +{ + }+, <{ w W n1 @ _ }>, <{ _ W n2 @ _ }>
-      => Some $ Expr.EBit w (BitArith.plus_mod w n1 n2) i
-    | +{ + }+, <{ w S z1 @ _ }>, <{ _ S z2 @ _ }>
-      => Some $ Expr.EInt w (IntArith.plus_mod w z1 z2) i
-    | +{ |+| }+, <{ w W n1 @ _ }>, <{ _ W n2 @ _ }>
-      => Some $ Expr.EBit w (BitArith.plus_sat w n1 n2) i
-    | +{ |+| }+,  <{ w S z1 @ _ }>, <{ _ S z2 @ _ }>
-      => Some $ Expr.EInt w (IntArith.plus_sat w z1 z2) i
-    | +{ - }+, <{ w W n1 @ _ }>, <{ _ W n2 @ _ }>
-      => Some $ Expr.EBit w (BitArith.minus_mod w n1 n2) i
-    | +{ - }+, <{ w S z1 @ _ }>, <{ _ S z2 @ _ }>
-      => Some $ Expr.EInt w (IntArith.minus_mod w z1 z2) i
-    | +{ |-| }+, <{ w W n1 @ _ }>, <{ _ W n2 @ _ }>
-      => Some $ Expr.EBit w (BitArith.minus_sat w n1 n2) i
-    | +{ |-| }+, <{ w S z1 @ _ }>, <{ _ S z2 @ _ }>
-      => Some $ Expr.EInt w (IntArith.minus_sat w z1 z2) i
-    | +{ × }+, <{ w W n1 @ _ }>, <{ _ W n2 @ _ }>
-      => Some $ Expr.EBit w (BitArith.mult_mod w n1 n2) i
-    | +{ × }+, <{ w S n1 @ _ }>, <{ _ S n2 @ _ }>
-      => Some $ Expr.EInt w (IntArith.mult_mod w n1 n2) i
-    | +{ << }+, <{ w W n1 @ _ }>, <{ _ W n2 @ _ }>
-      => Some $ Expr.EBit w (BitArith.shift_left w n1 n2) i
-    | +{ << }+, <{ w S z1 @ _ }>, <{ _ W z2 @ _ }>
-      => Some $ Expr.EInt w (IntArith.shift_left w z1 z2) i
-    | +{ >> }+, <{ w W n1 @ _ }>, <{ _ W n2 @ _ }>
-      => Some $ Expr.EBit w (BitArith.shift_right w n1 n2) i
-    | +{ >> }+, <{ w S z1 @ _ }>, <{ _ W z2 @ _ }>
-      => Some $ Expr.EInt w (IntArith.shift_right w z1 z2) i
-    | +{ & }+, <{ w W n1 @ _ }>, <{ _ W n2 @ _ }>
-      => Some $ Expr.EBit w (BitArith.bit_and w n1 n2) i
-    | +{ & }+, <{ w S z1 @ _ }>, <{ _ S z2 @ _ }>
-      => Some $ Expr.EInt w (IntArith.bit_and w z1 z2) i
-    | +{ ^ }+, <{ w W n1 @ _ }>, <{ _ W n2 @ _ }>
-      => Some $ Expr.EBit w (BitArith.bit_xor w n1 n2) i
-    | +{ ^ }+, <{ w S z1 @ _ }>, <{ _ S z2 @ _ }>
-      => Some $ Expr.EInt w (IntArith.bit_xor w z1 z2) i
-    | +{ | }+, <{ w W n1 @ _ }>, <{ _ W n2 @ _ }>
-      => Some $ Expr.EBit w (BitArith.bit_or w n1 n2) i
-    | +{ | }+, <{ w S z1 @ _ }>, <{ _ S z2 @ _ }>
-      => Some $ Expr.EInt w (IntArith.bit_or w z1 z2) i
-    | +{ <= }+, <{ w W n1 @ _ }>, <{ _ W n2 @ _ }> => Some $ Expr.EBool (n1 <=? n2)%Z i
-    | +{ <= }+, <{ w S z1 @ _ }>, <{ _ S z2 @ _ }> => Some $ Expr.EBool (z1 <=? z2)%Z i
-    | +{ < }+, <{ w W n1 @ _ }>, <{ _ W n2 @ _ }> => Some $ Expr.EBool (n1 <? n2)%Z i
-    | +{ < }+, <{ w S z1 @ _ }>, <{ _ S z2 @ _ }> => Some $ Expr.EBool (z1 <? z2)%Z i
-    | +{ >= }+, <{ w W n1 @ _ }>, <{ _ W n2 @ _ }> => Some $ Expr.EBool (n2 <=? n1)%Z i
-    | +{ >= }+, <{ w S z1 @ _ }>, <{ _ S z2 @ _ }> => Some $ Expr.EBool (z2 <=? z1)%Z i
-    | +{ > }+, <{ w W n1 @ _ }>, <{ _ W n2 @ _ }> => Some $ Expr.EBool (n2 <? n1)%Z i
-    | +{ > }+, <{ w S z1 @ _ }>, <{ _ S z2 @ _ }> => Some $ Expr.EBool (z2 <? z1)%Z i
-    | +{ && }+, <{ BOOL b1 @ _ }>, <{ BOOL b2 @ _ }> => Some $ Expr.EBool (b1 && b2) i
-    | +{ || }+, <{ BOOL b1 @ _ }>, <{ BOOL b2 @ _ }> => Some $ Expr.EBool (b1 || b2) i
-    | +{ == }+, _, _ => Some $ Expr.EBool (ExprEquivalence.eqbe v1 v2) i
-    | +{ != }+, _, _ => Some $ Expr.EBool (negb $ ExprEquivalence.eqbe v1 v2) i
-    | +{ ++ }+, <{ w1 W n1 @ _ }>, <{ w2 W n2 @ _ }>
-      => Some $ Expr.EBit (w1 + w2)%N (BitArith.concat w1 w2 n1 n2) i
-    | +{ ++ }+, <{ w1 W n1 @ _ }>, <{ w2 S n2 @ _ }>
-      => Some $ Expr.EBit (w1 + Npos w2)%N (BitArith.concat w1 (Npos w2) n1 n2) i
-    | +{ ++ }+, <{ w1 S n1 @ _ }>, <{ w2 S n2 @ _ }>
-      => Some $ Expr.EInt (w1 + w2)%positive (IntArith.concat (Npos w1) (Npos w2) n1 n2) i
-    | +{ ++ }+, <{ w1 S n1 @ _ }>, <{ w2 W n2 @ _ }>
-      =>
-      match w2 with
-      | 0%N => 
-        Some (Expr.EInt w1 n1 i)
-      | Npos w2 =>
-        Some $ Expr.EInt (w1 + w2)%positive (IntArith.concat (Npos w1) (Npos w2) n1 n2) i
-      end
+    | `+%bop, w `W n1, _ `W n2
+      => Some $ Expr.Bit w $ BitArith.plus_mod w n1 n2
+    | `+%bop, w `S z1, _ `S z2
+      => Some $ Expr.Int w $ IntArith.plus_mod w z1 z2
+    | |+|%bop, w `W n1, _ `W n2
+      => Some $ Expr.Bit w $ BitArith.plus_sat w n1 n2
+    | |+|%bop,  w `S z1, _ `S z2
+      => Some $ Expr.Int w $ IntArith.plus_sat w z1 z2
+    | `-%bop, w `W n1, _ `W n2
+      => Some $ Expr.Bit w $ BitArith.minus_mod w n1 n2
+    | `-%bop, w `S z1, _ `S z2
+      => Some $ Expr.Int w $ IntArith.minus_mod w z1 z2
+    | |-|%bop, w `W n1, _ `W n2
+      => Some $ Expr.Bit w $ BitArith.minus_sat w n1 n2
+    | |-|%bop, w `S z1, _ `S z2
+      => Some $ Expr.Int w $ IntArith.minus_sat w z1 z2
+    | ×%bop, w `W n1, _ `W n2
+      => Some $ Expr.Bit w $ BitArith.mult_mod w n1 n2
+    | ×%bop, w `S n1, _ `S n2
+      => Some $ Expr.Int w $ IntArith.mult_mod w n1 n2
+    | <<%bop, w `W n1, _ `W n2
+      => Some $ Expr.Bit w $ BitArith.shift_left w n1 n2
+    | <<%bop, w `S z1, _ `W z2
+      => Some $ Expr.Int w $ IntArith.shift_left w z1 z2
+    | >>%bop, w `W n1, _ `W n2
+      => Some $ Expr.Bit w $ BitArith.shift_right w n1 n2
+    | >>%bop, w `S z1, _ `W z2
+      => Some $ Expr.Int w $ IntArith.shift_right w z1 z2
+    | &%bop, w `W n1, _ `W n2
+      => Some $ Expr.Bit w $ BitArith.bit_and w n1 n2
+    | &%bop, w `S z1, _ `S z2
+      => Some $ Expr.Int w $ IntArith.bit_and w z1 z2
+    | ^%bop, w `W n1, _ `W n2
+      => Some $ Expr.Bit w $ BitArith.bit_xor w n1 n2
+    | ^%bop, w `S z1, _ `S z2
+      => Some $ Expr.Int w $ IntArith.bit_xor w z1 z2
+    | Expr.BitOr, w `W n1, _ `W n2
+      => Some $ Expr.Bit w $ BitArith.bit_or w n1 n2
+    | Expr.BitOr, w `S z1, _ `S z2
+      => Some $ Expr.Int w $ IntArith.bit_or w z1 z2
+    | ≤%bop, w `W n1, _ `W n2 => Some $ Expr.Bool (n1 <=? n2)%Z
+    | ≤%bop, w `S z1, _ `S z2 => Some $ Expr.Bool (z1 <=? z2)%Z
+    | `<%bop, w `W n1, _ `W n2 => Some $ Expr.Bool (n1 <? n2)%Z
+    | `<%bop, w `S z1, _ `S z2 => Some $ Expr.Bool (z1 <? z2)%Z
+    | ≥%bop, w `W n1, _ `W n2 => Some $ Expr.Bool (n2 <=? n1)%Z
+    | ≥%bop, w `S z1, _ `S z2 => Some $ Expr.Bool (z2 <=? z1)%Z
+    | `>%bop, w `W n1, _ `W n2 => Some $ Expr.Bool (n2 <? n1)%Z
+    | `>%bop, w `S z1, _ `S z2 => Some $ Expr.Bool (z2 <? z1)%Z
+    | `&&%bop, Expr.Bool b1, Expr.Bool b2 => Some $ Expr.Bool (b1 && b2)
+    | `||%bop, Expr.Bool b1, Expr.Bool b2 => Some $ Expr.Bool (b1 || b2)
+    | `==%bop, _, _ => Some $ Expr.Bool $ eqbe v1 v2
+    | !=%bop, _, _ => Some $ Expr.Bool $ negb $ eqbe v1 v2
+    | `++%bop, w1 `W n1, w2 `W n2
+      => Some $ Expr.Bit (w1 + w2)%N $ BitArith.concat w1 w2 n1 n2
+    | `++%bop, w1 `W n1, w2 `S n2
+      => Some $ Expr.Bit (w1 + Npos w2)%N $ BitArith.concat w1 (Npos w2) n1 n2
+    | `++%bop, w1 `S n1, w2 `S n2
+      => Some $ Expr.Int (w1 + w2)%positive $ IntArith.concat (Npos w1) (Npos w2) n1 n2
+    | `++%bop, w1 `S n1, w2 `W n2
+      => match w2 with
+        | 0%N => 
+            Some $ Expr.Int w1 n1
+        | Npos w2 =>
+            Some
+              $ Expr.Int (w1 + w2)%positive
+              $ IntArith.concat (Npos w1) (Npos w2) n1 n2
+        end
     | _, _, _ => None
     end.
-  (**[]*)
-  
-  (** Get header stack data from value. *)
-  Definition header_stack_data (v : Expr.e tags_t)
-    : option (Z * F.fs string (Expr.t) * (list (Expr.e tags_t))) :=
-    match v with
-    | <{ Stack hs:ts nextIndex:=ni @ _}> => Some (ni,ts,hs)
-    | _ => None
-    end.
-  (**[]*)
-  
-  Definition eval_member (x : string) (v : Expr.e tags_t) : option (Expr.e tags_t) :=
-    match v with
-    | <{ struct { vs } @ _ }>
-    | <{ hdr { vs } valid:=_ @ _ }> => vs ▷ F.get x
-    | _                             => None
-    end.
-  (**[]*)
-
-  (** Header stack access. *)
-  Definition eval_access (v : Expr.e tags_t) (n : Z) : option (Expr.e tags_t) :=
-    v
-      ▷ header_stack_data
-      >>| triple_3
-      >>= (fun hs => nth_error hs (Z.to_nat n)).
   
   Section Edefault.
     Local Hint Constructors value : core.
     
-    Fail Lemma value_edefault : forall i τ, value (edefault i τ).
-    (*Proof.
-      induction τ using custom_t_ind; unravel; auto 1;
-        try (constructor; apply repeat_Forall); constructor; auto 1;
-          try (ind_list_predfs; unfold F.predfs_data in * );
-          try ind_list_Forall; unravel in *; auto 4.
-    Qed. *)   
+    Lemma value_e_of_t : forall τ e,
+        e_of_t τ = Some e -> value e.
+    Proof.
+      intro t;
+        induction t using custom_t_ind;
+        intros e h; unravel in *; try discriminate;
+        try (inv h; auto; assumption).
+      destruct (sequence (map e_of_t ts))
+        as [es |] eqn:hseq; try discriminate.
+      inv h. constructor.
+      rewrite <- Forall2_sequence_iff in hseq.
+      rewrite <- Forall2_map_l in hseq.
+      eauto using Forall2_Forall_impl_Forall.
+    Qed.
   End Edefault.
   
   Section HelpersType.
-    Local Hint Constructors check_expr : core.
+    Local Hint Constructors type_expr : core.
     Local Hint Extern 0 => bit_bounded : core.
     Local Hint Extern 0 => int_bounded : core.
     
     Import CanonicalForms.
     
-    Lemma eval_slice_types : forall D Γ v v' τ hi lo w,
+    Lemma eval_slice_types : forall Γ v v' τ hi lo w,
         eval_slice hi lo v = Some v' ->
         value v ->
         (Npos lo <= Npos hi < w)%N ->
         numeric_width w τ ->
-        ⟦ D, Γ ⟧ ⊢ v ∈ τ ->
-        let w' := (Npos hi - Npos lo + 1)%N in
-        ⟦ D, Γ ⟧ ⊢ v' ∈ bit<w'>.
+        Γ ⊢ₑ v ∈ τ ->
+        Γ ⊢ₑ v' ∈ Expr.TBit (Npos hi - Npos lo + 1)%N.
     Proof.
-      intros D Γ v v' τ hi lo w Heval Hv Hw Hnum Ht w'; subst w';
-        inv Hnum; assert_canonical_forms; unravel in *; inv Heval; auto 2.
-    Admitted.
+      intros Γ v v' τ hi lo w Heval Hv Hw Hnum Ht; inv Hnum;
+        assert_canonical_forms; simpl in Heval;
+        unfold "$" in Heval; inv Heval; auto.
+    Qed.
     
     Local Hint Resolve BitArith.bound0 : core.
     Local Hint Resolve IntArith.bound0 : core.
     
-    Lemma eval_cast_types : forall D Γ τ τ' v v',
+    Lemma eval_cast_types : forall Γ τ τ' v v',
         eval_cast τ' v = Some v' ->
         value v ->
         proper_cast τ τ' ->
-        ⟦ D, Γ ⟧ ⊢ v ∈ τ ->
-        ⟦ D, Γ ⟧ ⊢ v' ∈ τ'.
+        Γ ⊢ₑ v ∈ τ ->
+        Γ ⊢ₑ v' ∈ τ'.
     Proof.
-      intros D Γ τ τ' v v' Heval Hv Hpc Ht;
+      intros Γ τ τ' v v' Heval Hv Hpc Ht;
         inv Hpc; assert_canonical_forms; unravel in *;
-          try match goal with
-              | H: context [ if ?b then _ else _ ]
-                |- _ => destruct b eqn:?
-              end; try (inv Heval; auto 2; assumption).
+        try match goal with
+            | H: context [ if ?b then _ else _ ]
+              |- _ => destruct b eqn:?
+            end; try (inv Heval; auto 2; assumption).
       - destruct x; try (inv Heval; auto 2; assumption).
         inv Heval; auto 2.
         constructor.
         unfold BitArith.bound.
         unfold BitArith.upper_bound.
         lia.
-    Admitted.
+      - destruct x; inv Heval; auto.
+        destruct p; inv H1; auto.
+      - destruct w; inv Heval; auto.
+      - destruct w2; inv Heval; auto.
+        destruct p; inv H1; auto.
+    Qed.
     
-        (*
-      - destruct w; inv Heval; auto 2.
-      - destruct w2; inv Heval; auto 2.
-      - inv Heval. constructor.
-        generalize dependent fs.
-        ind_list_Forall; intros [| [? ?] ?] ?;
-                                unravel in *; try inv_Forall2_cons;
-          constructor; try split;
-            unravel; try apply IHx; auto 2. (*
-      - inv Heval; constructor; auto 1.
-        + apply pn_header. rewrite F.predfs_data_map. assumption.
-        + clear x0 H0. generalize dependent fs.
-          ind_list_Forall; intros [| [? ?] ?] ? ;
-            unravel in *; try inv_Forall2_cons;
-              constructor; try split;
-                unravel; try apply IHx; auto 2.
-         *) *)
-    
-    Lemma eval_bop_types : forall Γ D op τ1 τ2 τ (i : tags_t) v1 v2 v,
+    Lemma eval_bop_types : forall Γ op τ1 τ2 τ v1 v2 v,
         bop_type op τ1 τ2 τ ->
         value v1 -> value v2 ->
-        eval_bop op v1 v2 i = Some v ->
-        ⟦ D, Γ ⟧ ⊢ v1 ∈ τ1 -> ⟦ D, Γ ⟧ ⊢ v2 ∈ τ2 -> ⟦ D, Γ ⟧ ⊢ v ∈ τ.
+        eval_bop op v1 v2 = Some v ->
+        Γ ⊢ₑ v1 ∈ τ1 -> Γ ⊢ₑ v2 ∈ τ2 -> Γ ⊢ₑ v ∈ τ.
     Proof.
-      intros Γ D op τ1 τ2 τ v1 v2 v i Hbop Hv1 Hv2 Heval Ht1 Ht2;
+      intros Γ op τ1 τ2 τ v1 v2 v Hbop Hv1 Hv2 Heval Ht1 Ht2;
         inv Hbop; unravel in *; try inv_numeric;
-          repeat assert_canonical_forms;
-          try (inv_numeric_width; assert_canonical_forms);
-          try (inv Heval; auto 2; assumption).
+        repeat assert_canonical_forms;
+        try (inv_numeric_width; assert_canonical_forms);
+        try (inv Heval; auto 2; assumption).
     Qed.
     
-    Lemma eval_member_types : forall D Γ x v v' ts τ τ',
-        eval_member x v = Some v' ->
+    Lemma eval_member_types : forall Γ x vs v ts τ,
+        nth_error ts x = Some τ ->
+        nth_error vs x = Some v ->
         value v ->
-        member_type ts τ ->
-        F.get x ts = Some τ' ->
-        ⟦ D, Γ ⟧ ⊢ v ∈ τ ->
-        ⟦ D, Γ ⟧ ⊢ v' ∈ τ'.
+        Forall2 (type_expr Γ) vs ts ->
+        Γ ⊢ₑ v ∈ τ.
     Proof.
-      intros D Γ x v v' ts τ τ' Heval Hv Hmem Hget Ht;
-        inv Hmem; assert_canonical_forms.
-      - eapply F.relfs_get_r in H1 as [? [? ?]]; eauto 2;
-          unravel in *; rewrite H in Heval;
-            unravel in *; inv Heval; intuition.
-      - eapply F.relfs_get_r in H6 as [? [? ?]]; eauto 2;
-          unravel in *; rewrite H in Heval;
-            unravel in *; inv Heval; intuition.
+      intros Γ x vs v ts t hntht hnthv hv hvsts.
+      rewrite Forall2_forall_nth_error in hvsts.
+      destruct hvsts as [_ hvt]; eauto.
     Qed.
     
-    Local Hint Constructors proper_nesting : core.
-    Hint Rewrite repeat_length.
-    Local Hint Resolve proper_inside_header_nesting : core.
     Local Hint Resolve BitArith.bound0 : core.
     Local Hint Resolve IntArith.bound0 : core.
     
-    Fail Lemma edefault_types : forall D Γ i τ,
-        PT.proper_nesting τ ->
-        let e := edefault i τ in
-        ⟦ D, Γ ⟧ ⊢ e ∈ τ.
-    (*Proof.
-      intros; subst e; induction τ using custom_t_ind; unravel;
-        invert_proper_nesting; auto 2;
-          constructor; autorewrite with core; auto 2;
-            try (apply repeat_Forall; constructor; auto 2);
-            try (ind_list_Forall; repeat inv_Forall_cons; constructor; intuition);
-            try (ind_list_predfs; repeat invert_cons_predfs; constructor;
-                 try split; unravel; intuition).
-                 Qed.*)
+    Lemma e_of_t_types : forall Γ τ e,
+        e_of_t τ = Some e -> Γ ⊢ₑ e ∈ τ.
+    Proof.
+      intros Γ t; induction t using custom_t_ind;
+        unravel in *; intros e h; try discriminate.
+      - inv h; auto.
+      - inv h; auto.
+      - inv h; auto.
+      - inv h; auto.
+      - destruct (sequence (map e_of_t ts)) as [es |] eqn:hes;
+          try discriminate; inv h.
+        rewrite <- Forall2_sequence_iff in hes.
+        rewrite <- Forall2_map_l in hes.
+        constructor;
+          eauto using Forall2_Forall_impl_Forall.
+        + destruct b; auto.
+        + assert (hlen: length ts = length es)
+            by eauto using Forall2_length.
+          pose proof Forall_specialize_Forall2
+               _ _ _ _ H _ hlen as h; clear H hlen.
+          rewrite Forall2_flip.
+          pose proof Forall2_impl _ _ _ _ _ _ h hes; eauto.
+    Qed.
     
     Local Hint Resolve Forall_impl : core.
-    Local Hint Resolve Forall_firstn : core.
-    Local Hint Resolve Forall_skipn : core.
-    Local Hint Resolve proper_inside_header_nesting : core.
-    Fail Local Hint Resolve edefault_types : core.
+    Local Hint Resolve e_of_t_types : core.
     Hint Rewrite app_length.
     Hint Rewrite Forall_app.
-    Hint Rewrite firstn_length_le.
-    Hint Rewrite skipn_length.
     Hint Rewrite map_length.
-    Hint Rewrite (@F.predfs_data_map string).
-    Hint Rewrite @F.map_fst.
-    Hint Rewrite @map_compose.
-    Hint Rewrite (@Forall2_map_l Expr.t).
-    Hint Rewrite (@Forall2_Forall Expr.t).
-    Hint Rewrite (@F.predfs_data_map).
-    Hint Rewrite @F.relfs_split_map_iff.
-    Hint Rewrite @F.map_snd.
     
-    Lemma eval_uop_types : forall D Γ op e v τ τ',
+    Lemma eval_uop_types : forall Γ op e v τ τ',
         uop_type op τ τ' -> value e -> eval_uop op e = Some v ->
-        ⟦ D, Γ ⟧ ⊢ e ∈ τ -> ⟦ D, Γ ⟧ ⊢ v ∈ τ'.
-    (*Proof.
-      intros D Γ op e v τ τ' Huop Hev Heval Het;
+        Γ ⊢ₑ e ∈ τ -> Γ ⊢ₑ v ∈ τ'.
+    Proof.
+      intros Γ op e v τ τ' Huop Hev Heval Het;
         inv Huop; try inv_numeric;
-          assert_canonical_forms; unravel in *;
-            inv Heval; auto 2; invert_proper_nesting;
-              repeat match goal with
+        assert_canonical_forms; unravel in *;
+        inv Heval; auto 2;
+        repeat match goal with
                      | H: (if ?b then _ else _) = Some _
                        |- _ => destruct b as [? | ?] eqn:?
-                     | H: Some _ = Some _ |- _ => inv H
-                     end; eauto 2;
-                try constructor; auto 2; try (destruct n; lia);
-                  autorewrite with core; try lia;
-                    try split; auto 2;
-                      try (apply repeat_Forall; constructor; auto 2;
-                           autorewrite with core in *; split; [intuition | unravel; eauto 5]).
-      - eapply Forall_nth_error in H9; eauto 1; simpl in *; auto 1.
-    Qed.*)
-    Admitted.
+               | H: Some _ = Some _ |- _ => inv H
+               end; eauto 2.
+      destruct x0; inv H1; auto.
+    Qed.
   End HelpersType.
   
   Section HelpersExist.
     Import CanonicalForms.
     
-    Lemma eval_slice_exists : forall D Γ v τ hi lo w,
+    Lemma eval_slice_exists : forall Γ v τ hi lo w,
         value v ->
         (Npos lo <= Npos hi < w)%N ->
         numeric_width w τ ->
-        ⟦ D, Γ ⟧ ⊢ v ∈ τ ->
+        Γ ⊢ₑ v ∈ τ ->
         exists v', eval_slice hi lo v = Some v'.
     Proof.
-      intros D Γ v τ hi lo w Hv Hw Hnum Ht;
+      intros Γ v τ hi lo w Hv Hw Hnum Ht;
         inv Hnum; assert_canonical_forms; unravel; eauto 2.
     Qed.
     
-    Lemma eval_cast_exists : forall D Γ e τ τ',
+    Lemma eval_cast_exists : forall Γ e τ τ',
         value e ->
         proper_cast τ τ' ->
-        ⟦ D, Γ ⟧ ⊢ e ∈ τ ->
+        Γ ⊢ₑ e ∈ τ ->
         exists v, eval_cast τ' e = Some v.
     Proof.
-      intros ? ? ? ? ? Hv Hpc Het; inv Hpc; assert_canonical_forms;
+      intros ? ? ? ? Hv Hpc Het; inv Hpc; assert_canonical_forms;
         unravel; simpl in *; eauto 2.
       - destruct x; eauto 2.
       - destruct x; eauto 2; destruct p; eauto 2;
           try (cbv in H0; destruct H0; try destruct p; discriminate).
       - destruct w; eauto 2.
       - destruct w2; eauto 2.
-    Admitted.
+        destruct p; eauto.
+    Qed.
     
-    Lemma eval_bop_exists : forall D Γ op τ1 τ2 τ (i : tags_t) v1 v2,
+    Lemma eval_bop_exists : forall Γ op τ1 τ2 τ v1 v2,
         bop_type op τ1 τ2 τ ->
         value v1 -> value v2 ->
-        ⟦ D, Γ ⟧ ⊢ v1 ∈ τ1 -> ⟦ D, Γ ⟧ ⊢ v2 ∈ τ2 ->
-        exists v, eval_bop op v1 v2 i = Some v.
+        Γ ⊢ₑ v1 ∈ τ1 -> Γ ⊢ₑ v2 ∈ τ2 ->
+        exists v, eval_bop op v1 v2 = Some v.
     Proof.
-      intros D Γ op τ1 τ2 τ i v1 v2 Hbop Hv1 Hv2 Ht1 Ht2;
+      intros Γ op τ1 τ2 τ v1 v2 Hbop Hv1 Hv2 Ht1 Ht2;
         inv Hbop; try inv_numeric; try inv_numeric_width;
           repeat assert_canonical_forms; unravel; eauto 2.
     Qed.
     
-    Lemma eval_uop_exists : forall op D Γ e τ τ',
-        uop_type op τ τ' -> value e -> ⟦ D, Γ ⟧ ⊢ e ∈ τ ->
+    Lemma eval_uop_exists : forall op Γ e τ τ',
+        uop_type op τ τ' -> value e -> Γ ⊢ₑ e ∈ τ ->
         exists v, eval_uop op e = Some v.
-    (* Proof.
-      intros op D Γ e τ τ' Hu Hv Het; inv Hu;
-        try inv_numeric; assert_canonical_forms;
-          unravel; eauto 2.
-      - assert (Hnihs : (Z.to_nat x0 < length x)%nat) by lia.
-        pose proof nth_error_exists _ _ Hnihs as [? Hnth].
-        rewrite Hnth; eauto 2.
-      - destruct (lt_dec (Pos.to_nat p) (Pos.to_nat n)) as [? | ?]; eauto 2.
-      - destruct (lt_dec (Pos.to_nat p) (Pos.to_nat n)) as [? | ?]; eauto 2.
-    Qed. *)
-    Admitted.
-      
-    Lemma eval_member_exists : forall D Γ x v ts τ τ',
-        value v ->
-        member_type ts τ ->
-        F.get x ts = Some τ' ->
-        ⟦ D, Γ ⟧ ⊢ v ∈ τ ->
-        exists v', eval_member x v = Some v'.
     Proof.
-      intros D Γ x v ts τ τ' Hv Hmem Hget Ht;
-        inv Hmem; assert_canonical_forms; unravel.
-      - eapply F.relfs_get_r in H1 as [? [? ?]]; eauto 2;
-          unravel in *; rewrite H; unravel; eauto 2.
-      - eapply F.relfs_get_r in H6 as [? [? ?]]; eauto 2;
-          unravel in *; rewrite H; unravel; eauto 2.
+      intros op Γ e τ τ' Hu Hv Het; inv Hu;
+        try inv_numeric; assert_canonical_forms;
+        unravel; eauto 2.
+      destruct x0; try contradiction; eauto.
+    Qed.
+      
+    Lemma eval_member_exists : forall Γ x vs ts τ,
+        Forall value vs ->
+        Forall2 (type_expr Γ) vs ts ->
+        nth_error ts x = Some τ ->
+        exists v, nth_error vs x = Some v.
+    Proof.
+      intros Γ x vs ts t hv h hnth.
+      apply nth_error_exists.
+      apply Forall2_length in h.
+      rewrite h.
+      eauto using ForallMap.nth_error_some_length.
     Qed.
   End HelpersExist.
   
   (** Lookup an lvalue. *)
-  Fixpoint lv_lookup (ϵ : eenv) (lv : Expr.e tags_t) : option (Expr.e tags_t) :=
+  Fixpoint lv_lookup (ϵ : list Expr.e) (lv : Expr.e) : option Expr.e :=
     match lv with
-    | <{ Var x:_ @ _ }> => ϵ x
-    | <{ Mem lv dot x : _ @ _ }> =>
-      (* TODO: use monadic bind. *)
-      match lv_lookup ϵ lv with
-      | Some <{ struct { fs } @ _ }>
-      | Some <{ hdr { fs } valid:=_  @ _ }> => fs ▷ F.get x
-      | _ => None
-      end
-    | <{ Access lv[n] : _ @ _ }> =>
-      match lv_lookup ϵ lv with
-      | Some <{ Stack vss:_ nextIndex:=_ @ _ }> => nth_error vss (Z.to_nat n)
-      | _ => None
-      end
+    | Expr.Var _ x => nth_error ϵ x
+    | Expr.Member _ x lv
+      => match lv_lookup ϵ lv with
+        | Some (Expr.Struct fs _) => nth_error fs x
+        | _ => None
+        end
+    | Expr.Slice lv hi lo => lv_lookup ϵ lv >>= eval_slice hi lo
     | _ => None
     end.
-  (**[]*)
   
   (** Updating an lvalue in an environment. *)
-  Fixpoint lv_update (lv v : Expr.e tags_t) (ϵ : eenv) : eenv :=
+  Fixpoint lv_update (lv v : Expr.e) (ϵ : list Expr.e) : list Expr.e :=
     match lv with
-    | <{ Var x:_ @ _ }> => ( x ↦ v ,, ϵ )
-    | <{ Mem lv dot x : _ @ _ }> =>
-      match lv_lookup ϵ lv with
-      | Some <{ struct { vs } @ i }>
-        => lv_update lv (Expr.EStruct (F.update x v vs) i) ϵ
-      | Some <{ hdr { vs } valid:=b @ i }>
-        => lv_update lv (Expr.EHeader (F.update x v vs) b i) ϵ
-      | _ => ϵ
-      end
-    | <{ Access lv[n] : _ @ _ }> =>
-      match lv_lookup ϵ lv with
-      | Some <{ Stack vss:ts nextIndex:=ni @ i }> =>
-        let vss := nth_update (Z.to_nat n) v vss in
-        lv_update lv <{ Stack vss:ts nextIndex:=ni @ i }> ϵ
-      | _ => ϵ
-      end
+    | Expr.Var _ x => nth_update x v ϵ
+    | Expr.Member _ x lv
+      => match lv_lookup ϵ lv with
+        | Some (Expr.Struct vs ob)
+          => lv_update lv (Expr.Struct (nth_update x v vs) ob) ϵ
+        | _ => ϵ
+        end
+    | Expr.Slice lv hi lo
+      => match v, lv_lookup ϵ lv with
+        | (Expr.Bit _ n | Expr.Int _ n), Some (w `W _)%expr =>
+            let rhs := N.shiftl (Z.to_N n) w in
+            let mask :=
+              Z.to_N
+                (-1 -
+                   (Z.of_N (N.lxor
+                              (N.pow 2 (Npos hi + 1) - 1)
+                              (N.pow 2 (Npos lo - 1))))) in
+            let new := Z.lxor (Z.land n (Z.of_N mask)) (Z.of_N rhs) in
+            lv_update lv (w `W new) ϵ
+        | _, _ => ϵ
+        end
     | _ => ϵ
     end.
-  (**[]*)
   
   (** Create a new environment
       from a closure environment where
@@ -503,7 +398,7 @@ Section StepDefs.
       into the function parameters. *)
   Definition copy_in
              (argsv : Expr.args tags_t)
-             (ϵcall : eenv) : eenv -> eenv :=
+             (ϵcall : (list Expr.e)) : (list Expr.e) -> (list Expr.e) :=
     F.fold (fun x arg ϵ =>
               match arg with
               | PAIn v     => ( x ↦ v ,, ϵ )
@@ -520,7 +415,7 @@ Section StepDefs.
       out variables from function call evaluation. *)
   Definition copy_out
              (argsv : Expr.args tags_t)
-             (ϵf : eenv) : eenv -> eenv :=
+             (ϵf : (list Expr.e)) : (list Expr.e) -> (list Expr.e) :=
     F.fold (fun x arg ϵ =>
               match arg with
               | PADirLess _ => ϵ (*what to do with directionless param*)
@@ -539,17 +434,17 @@ Section StepDefs.
   
   (** Function declarations and closures. *)
   Inductive fdecl : Type :=
-  | FDecl (closure : eenv) (fs : fenv) (ins : ienv) (body : Stmt.s tags_t)
+  | FDecl (closure : (list Expr.e)) (fs : fenv) (ins : ienv) (body : Stmt.s tags_t)
   with fenv : Type :=
   | FClmt (fs : Clmt.t string fdecl)
   (** Action declarations and closures *)
   with adecl : Type :=
-  | ADecl (closure : eenv) (fs : fenv) (ins : ienv) (aa : aenv) (body : Stmt.s tags_t)
+  | ADecl (closure : (list Expr.e)) (fs : fenv) (ins : ienv) (aa : aenv) (body : Stmt.s tags_t)
   with aenv : Type :=
   | AClmt (aa : Clmt.t string adecl)
   (** Instances and Clmtironment. *)
   with inst : Type :=
-  | CInst (closure : eenv) (fs : fenv) (ins : ienv)
+  | CInst (closure : (list Expr.e)) (fs : fenv) (ins : ienv)
           (tbls : tenv) (aa : aenv)
           (apply_blk : Stmt.s tags_t)  (* control instance *)
   | PInst (* TODO: parser instance *)
@@ -585,7 +480,7 @@ Section StepDefs.
   (** Control plane table entries,
       essentially mapping tables to an action call. *)
   Definition entries : Type :=
-    list (Expr.e tags_t * Expr.matchkind) ->
+    list (Expr.e * Expr.matchkind) ->
     list string ->
     string * Expr.args tags_t.
   (**[]*)
@@ -595,7 +490,7 @@ Section StepDefs.
   
   (** Control declarations and closures. *)
   Inductive cdecl : Type :=
-  | CDecl (cs : cenv) (closure : eenv) (fs : fenv) (ins : ienv)
+  | CDecl (cs : cenv) (closure : (list Expr.e)) (fs : fenv) (ins : ienv)
           (body : Control.d tags_t) (apply_block : Stmt.s tags_t)
   with cenv : Type :=
   | CClmt (cs : Clmt.t string cdecl).
